rearrange Gencot array lemmas

isa/Gencot_CArray_Lemmas.thy
@@ -2,22 +2,35 @@ theory Gencot_CArray_Lemmas
   imports "Gencot_CArray_Tuples"
 begin
 
-text \<open>Lift arrays to the wrapper records.
-      We introduce an overloaded abstract data type for all such arrays with indexes of type nat.
-      It consists of the following functions.
-      Array accesses are always guarded by function vld.\<close>
+section "Support for Reasoning with C Arrays"
+
+text \<open>
+We introduce an overloaded abstract data type for all C arrays with 
+indexes of type nat. It consists of two selector functions and two constructor
+functions which reflect the main ways how to work with arrays in C.
+The second constructor comes in two variants for either fixed size arrays 
+or variable sized arrays.
+\<close>
 consts 
-  arr :: "'el list \<Rightarrow> 'arr"
   siz :: "'arr \<Rightarrow> nat"
-  vld :: "'arr \<Rightarrow> nat \<Rightarrow> bool"
   elm :: "nat \<Rightarrow> 'arr \<Rightarrow> 'el"
   elm_update :: "nat \<Rightarrow> ('el \<Rightarrow> 'el) \<Rightarrow> 'arr \<Rightarrow> 'arr"
-  elm_modified :: "nat \<Rightarrow> ('el \<Rightarrow> 'el \<Rightarrow> bool) \<Rightarrow> 'arr \<Rightarrow> 'arr \<Rightarrow> bool"
-  arr_fill :: "(nat \<Rightarrow> 'el) \<Rightarrow> 'arr"
+  elms_fill :: "(nat \<Rightarrow> 'el) \<Rightarrow> 'arr"
+  elms_fill_n :: "nat \<Rightarrow> (nat \<Rightarrow> 'el) \<Rightarrow> 'arr"
 
-text \<open>For every actual wrapper record the following locale will be interpreted.
-      It extends CArrFuns by the laws of the abstract data type, 
-      and conversion from the Gencot array functions to the abstract data type functions.\<close>
+text \<open>
+Additionally we define derived functions as abbreviations for typical use cases.
+\<close>
+consts
+  vld :: "'arr \<Rightarrow> nat \<Rightarrow> bool"
+  elm_modified :: "nat \<Rightarrow> ('el \<Rightarrow> 'el \<Rightarrow> bool) \<Rightarrow> 'arr \<Rightarrow> 'arr \<Rightarrow> bool"
+
+subsection "Fixed Sized Arrays"
+
+text \<open>
+For every actual wrapper record (i.e., array size) the following locale 
+will be interpreted. It extends CArrFuns by the laws of the abstract data type, 
+and semantics theorems for the Gencot array operations.\<close>
 
 locale CArrLems = CArrFuns fld wrp
   for 
@@ -30,24 +43,30 @@ begin
 
 text \<open>Define conversion functions between lists and the wrapper record.\<close>
 definition lstFxd :: "'arr \<Rightarrow> 'el list"
-  where "lstFxd a \<equiv> Rep_FixedList (fld a)"
+  where lstFxd_def[simp]: "lstFxd a \<equiv> Rep_FixedList (fld a)"
 definition arrFxd :: "'el list \<Rightarrow> 'arr"
-  where "arrFxd a \<equiv> wrp (Abs_FixedList a)"
+  where arrFxd_def[simp]: "arrFxd a \<equiv> wrp (Abs_FixedList a)"
 
 text \<open>Define the abstract data type functions for the wrapper record.\<close>
 definition sizFxd :: "'arr \<Rightarrow> nat"
   where "sizFxd a \<equiv> length (lstFxd a)"
-definition vldFxd :: "'arr \<Rightarrow> nat \<Rightarrow> bool"
-  where "vldFxd a i \<equiv> i < sizFxd a"
 definition elmFxd :: "nat \<Rightarrow> 'arr \<Rightarrow> 'el"
   where "elmFxd i a \<equiv> nth (lstFxd a) i"
 definition elm_updateFxd :: "nat \<Rightarrow> ('el \<Rightarrow> 'el) \<Rightarrow> 'arr \<Rightarrow> 'arr"
-  where "elm_updateFxd i f a \<equiv> arrFxd (list_update (lstFxd a) i (f (elmFxd i a)))"
+  (* Define elm_updateFxd as total, so that elm_distUpd needs no assumption *)
+  where "elm_updateFxd i f a \<equiv> 
+    if i < LENGTH('n) then arrFxd (list_update (lstFxd a) i (f (elmFxd i a))) else a"
+definition elms_fillFxd :: "(nat \<Rightarrow> 'el) \<Rightarrow> 'arr"
+  where "elms_fillFxd f \<equiv> arrFxd [f x . x \<leftarrow> [0 ..< LENGTH('n)]]"
+
+lemmas unfold = sizFxd_def elmFxd_def elm_updateFxd_def elms_fillFxd_def
+
+text \<open>Additional derived functions\<close>
+definition vldFxd :: "'arr \<Rightarrow> nat \<Rightarrow> bool"
+  where vldFxd_def[simp]: "vldFxd a i \<equiv> i < sizFxd a"
 definition elm_modifiedFxd :: "nat \<Rightarrow> ('el \<Rightarrow> 'el \<Rightarrow> bool) \<Rightarrow> 'arr \<Rightarrow> 'arr \<Rightarrow> bool"
   where elm_modified_def: "elm_modifiedFxd i m a1 a2 \<equiv> 
     m (elmFxd i a1) (elmFxd i a2) \<and> (\<forall>j \<noteq> i. vldFxd a1 j \<longrightarrow> elmFxd j a1 = elmFxd j a2)"
-definition arr_fillFxd :: "(nat \<Rightarrow> 'el) \<Rightarrow> 'arr"
-  where "arr_fillFxd f \<equiv> arrFxd [f x . x \<leftarrow> [0 ..< LENGTH('n)]]"
 
 text \<open>Arrays are never empty.\<close>
 lemma arrNotNil: "\<forall>x::'arr .  lstFxd x \<noteq> []"
@@ -56,101 +75,66 @@ lemma arrNotNil: "\<forall>x::'arr .  lstFxd x \<noteq> []"
   apply(cut_tac x = "(fld x)" in Rep_FixedList )
   by auto
 
-text \<open>Laws for the abstract data type functions\<close>
-lemma sizArr: "sizFxd a = LENGTH('n)"
+text \<open>Simplification rules for selectors siz and elm\<close>
+lemma sizArr[simp]: "sizFxd a = LENGTH('n)"
   apply(unfold sizFxd_def lstFxd_def)
   by (simp add: length_FixedList)
-lemma vldArr: "vldFxd a n = (n < LENGTH('n))"
-  by (simp add: vldFxd_def sizArr)
+lemma elmElmUpd[simp]: "vldFxd a i \<Longrightarrow> elmFxd i (elm_updateFxd i f a) = f (elmFxd i a)"
+  apply(simp add: unfold wrp_inverse)
+  apply(cut_tac x = "(fld a)" in Rep_FixedList )
+  by(simp add: Abs_FixedList_inverse)
+lemma elmElmsFill[simp]: "i < LENGTH('n) \<Longrightarrow> elmFxd i (elms_fillFxd f) = f i"
+  by(simp add: unfold wrp_inverse Abs_FixedList_inverse)
+lemma elmElmUpdFrame[simp]: "vldFxd a i \<and> vldFxd a j \<and> i \<noteq> j \<Longrightarrow> elmFxd j (elm_updateFxd i f a) = elmFxd j a"
+  apply(auto simp add: elm_updateFxd_def elmFxd_def)
+  apply(cut_tac x = "(fld a)" in Rep_FixedList )
+  apply(subst wrp_inverse)
+  apply(subst Abs_FixedList_inverse)
+  by (auto)
+
+text \<open>Reasoning rules for elm_update\<close>
 lemma elm_identUpd[simp]: "elm_updateFxd i (\<lambda>a. a) = (\<lambda>a. a)"
-  apply (unfold elm_updateFxd_def)
-  by(simp add: elmFxd_def arrFxd_def lstFxd_def Rep_FixedList_inverse fld_inverse)
+  by(auto simp add: unfold Rep_FixedList_inverse fld_inverse)
 lemma elm_sameUpd: "elm_updateFxd i (\<lambda>_. m (elmFxd i x)) x = elm_updateFxd i m x"
-  by(simp add: elm_updateFxd_def)
-lemma elm_distUpd: "(i < LENGTH('n)) \<Longrightarrow> (elm_updateFxd i f) \<circ> (elm_updateFxd i g) = elm_updateFxd i (f \<circ> g)"
+  by(simp add: unfold)
+lemma elm_distUpd: "(elm_updateFxd i f) \<circ> (elm_updateFxd i g) = elm_updateFxd i (f \<circ> g)"
   for f:: "'el \<Rightarrow> 'el"
-  apply (unfold elm_updateFxd_def elmFxd_def arrFxd_def lstFxd_def)
-  apply(rule ext,simp)
-  apply(cut_tac x = "(fld a)" in Rep_FixedList )
-  apply(subst wrp_inverse)+
-  apply(subst Abs_FixedList_inverse,simp)+
-  by(auto)
-lemma elm_commUpd_elm: "i < j \<Longrightarrow> (elm_updateFxd j m2) \<circ> (elm_updateFxd i m1) = (elm_updateFxd i m1) \<circ> (elm_updateFxd j m2)"
-  apply (unfold elm_updateFxd_def elmFxd_def arrFxd_def lstFxd_def)
-  apply(rule ext,simp)
+  apply(rule ext,simp add: unfold)
   apply(cut_tac x = "(fld x)" in Rep_FixedList )
-  apply(subst wrp_inverse)+
-  apply(subst Abs_FixedList_inverse,simp)+
-  apply (simp)
-  apply(rule arg_cong[where f=wrp])
-  apply(rule arg_cong[where f=Abs_FixedList])
-  apply(rule list_update_swap)
-  by(simp)
-lemma elmElmUpd: "vldFxd a i \<Longrightarrow> elmFxd i (elm_updateFxd i f a) = f (elmFxd i a)"
-  apply(auto simp add: elm_updateFxd_def elmFxd_def arrFxd_def lstFxd_def vldArr)
-  apply(cut_tac x = "(fld a)" in Rep_FixedList )
-  apply(subst wrp_inverse)
-  apply(subst Abs_FixedList_inverse)
-  by (auto)
-lemma elmElmUpdFrame: "vldFxd a i \<and> vldFxd a j \<and> i \<noteq> j \<Longrightarrow> elmFxd j (elm_updateFxd i f a) = elmFxd j a"
-  apply(auto simp add: elm_updateFxd_def elmFxd_def arrFxd_def lstFxd_def vldArr)
-  apply(cut_tac x = "(fld a)" in Rep_FixedList )
-  apply(subst wrp_inverse)
-  apply(subst Abs_FixedList_inverse)
-  by (auto)
-lemma elmArrFill: "i < LENGTH('n) \<Longrightarrow> elmFxd i (arr_fillFxd f) = f i"
-  apply(auto simp add: elmFxd_def arr_fillFxd_def lstFxd_def arrFxd_def wrp_inverse vldArr sizArr)
-  apply(subst Abs_FixedList_inverse)
-  by auto
+  by(simp add: wrp_inverse  Abs_FixedList_inverse)
+
+lemma elm_commUpd_elm: "i < j \<Longrightarrow> (elm_updateFxd j m2) \<circ> (elm_updateFxd i m1) = (elm_updateFxd i m1) \<circ> (elm_updateFxd j m2)"
+  apply(rule ext,simp add: unfold)
+  apply(cut_tac x = "(fld x)" in Rep_FixedList )
+  by(simp add: wrp_inverse Abs_FixedList_inverse list_update_swap)
 
 text \<open>Array equality by extensionality. \<close>
 lemma eqArr1: "(\<And> i. (vldFxd a1 i) \<Longrightarrow> ((elmFxd i a1) = (elmFxd i a2))) \<Longrightarrow> (a1 = a2)"
-  apply(auto simp add: elmFxd_def vldFxd_def sizFxd_def lstFxd_def)
-  apply(drule nth_equalityI[rotated])
-  apply(cut_tac x = "(fld a1)" in Rep_FixedList )
-  apply(cut_tac x = "(fld a2)" in Rep_FixedList )
-  apply(simp)
-  apply(drule arg_cong[where f = Abs_FixedList])
-  apply(subst (asm) Rep_FixedList_inverse)+
+  apply(unfold elmFxd_def vldFxd_def sizFxd_def lstFxd_def)
+  apply(drule nth_equalityI[rotated],simp add: length_FixedList)
+  apply(drule Rep_FixedList_inject[THEN iffD1])
   apply(drule arg_cong[where f = wrp])
-  apply(simp add: fld_inverse)
-  done
+  by(simp add: fld_inverse)
+
 lemma eqArr: "(a1 = a2) = 
               (\<forall> i. (vldFxd a1 i) \<longrightarrow> ((elmFxd i a1) = (elmFxd i a2)))"
-  apply(rule iffI)
-   apply(rule allI)
-   apply(rule impI)
-   apply(auto)
+  apply(rule iffI,simp)
   by (rule eqArr1,auto)
 
 lemma eqElmUpd: "vldFxd a2 i \<Longrightarrow> (a1 = elm_updateFxd i f a2) =
                  ((elmFxd i a1) = f (elmFxd i a2) \<and> (\<forall> j. j \<noteq> i \<and> (vldFxd a1 j) \<longrightarrow> (elmFxd j a1) = (elmFxd j a2)))"
-  apply(rule iffI)
-   apply(auto)
-    apply(subst elmElmUpd,auto)
-  apply(subst elmElmUpdFrame,auto simp add: vldArr)
-  apply(subst eqArr)
+  apply(rule iffI,simp)
+  apply(simp add: eqArr)
    apply(rule allI)
-  apply(rule impI)
   apply(case_tac "ia = i")
-  apply(simp)
-   apply(subst elmElmUpd,auto simp add: vldArr)
-  apply(subst elmElmUpdFrame,auto simp add: vldArr)
-  done
+  by(auto)
 
-lemma eqArrFill: "(a = arr_fillFxd f) = 
+lemma eqElmsFill: "(a = elms_fillFxd f) = 
                  ((\<forall> i. (vldFxd a i) \<longrightarrow> ((elmFxd i a) = f i)))"
-  apply(rule iffI)
-   apply(auto)
-   apply(rule elmArrFill)
-   apply(simp add: vldArr)
-  apply(subst eqArr)
-   apply(rule allI)
-   apply(rule impI)
-  apply(subst elmArrFill)
-  by (auto simp add: vldArr)
+  apply(rule iffI,simp)
+  by(simp add: eqArr)
 
-text \<open>Semantics theorems for the Gencot array functions.\<close>
+text \<open>Semantics theorems for the Gencot array operations.\<close>
 
 definition ctrct_getArrFxd :: "'arr \<times> ('m::len) word \<Rightarrow> bool"
   where ctrct_getArrFxd_def[simp]:
@@ -158,11 +142,11 @@ definition ctrct_getArrFxd :: "'arr \<times> ('m::len) word \<Rightarrow> bool"
 theorem sem_getArr: 
  "ctrct_getArrFxd (a,i) \<Longrightarrow> 
   getArrFxd (a,i) = elmFxd (unat i) a"
-  by (simp add: getArrFxd_def getArr'_def vldArr elmFxd_def lstFxd_def)
+  by (simp add: getArrFxd_def getArr'_def elmFxd_def)
 theorem errsem_getArr:
  "\<not> ctrct_getArrFxd (a,i) \<Longrightarrow> 
   getArrFxd (a,i) = elmFxd 0 a"
-  apply(simp add: getArrFxd_def getArr'_def vldArr elmFxd_def)
+  apply(simp add: getArrFxd_def getArr'_def elmFxd_def)
   apply(fold lstFxd_def)
   apply(case_tac " lstFxd a")
    apply(cut_tac arrNotNil)
@@ -174,190 +158,405 @@ definition ctrct_setArrFxd :: "'arr \<times> ('m::len) word \<times> 'el \<Right
 theorem sem_setArr: 
  "ctrct_setArrFxd (a,i,v) \<Longrightarrow> 
   setArrFxd (a,i,v) = (elm_updateFxd (unat i) (\<lambda>_.v) a, ())"
-  by (simp add: setArrFxd_def setArr'_def vldArr lstFxd_def arrFxd_def elm_updateFxd_def)
+  by (simp add: setArrFxd_def setArr'_def elm_updateFxd_def)
 theorem errsem_setArr:
  "\<not> ctrct_setArrFxd (a,i,v) \<Longrightarrow> 
   setArrFxd (a,i,v) = (a,())"
-  by (simp add: setArrFxd_def setArr'_def vldArr fld_inverse)
+  by (simp add: setArrFxd_def setArr'_def fld_inverse)
 
 definition ctrct_modifyArrFxd :: "'arr \<times> ('m::len) word \<times> ('el \<times> 'arg \<Rightarrow> 'el \<times> 'out) \<times> 'arg \<Rightarrow> bool"
   where ctrct_modifyArrFxd_def[simp]:
-  "ctrct_modifyArrFxd x \<equiv> let (a,i,f,v) = x in vldFxd a (unat i)"
+  "ctrct_modifyArrFxd x \<equiv> let (a,(i,f,v)) = x in vldFxd a (unat i)"
 theorem sem_modifyArr:
- "ctrct_modifyArrFxd (a,i,f,x) \<Longrightarrow> 
-  modifyArrFxd (a,i,f,x) = 
-  (let (e,y) = f (elmFxd (unat i) a, x) in (elm_updateFxd (unat i) (\<lambda>_.e) a, y))"
-  by (simp add: modifyArrFxd_def modifyArr'_def split_def Let_def vldArr lstFxd_def arrFxd_def elm_updateFxd_def elmFxd_def)
+ "ctrct_modifyArrFxd (a,x) \<Longrightarrow> 
+  modifyArrFxd (a,x) = 
+  (let (i,f,x) = x; (e,y) = f (elmFxd (unat i) a, x) in (elm_updateFxd (unat i) (\<lambda>_.e) a, y))"
+  by (simp add: modifyArrFxd_def modifyArr'_def split_def Let_def elm_updateFxd_def elmFxd_def)
 theorem errsem_modifyArr:
- "\<not> ctrct_modifyArrFxd (a,i,f,x) ==> 
-  modifyArrFxd (a,i,f,x) = modifyArrFxd (a,0,f,x)"
-  by (simp add: modifyArrFxd_def modifyArr'_def vldArr fld_inverse)
+ "\<not> ctrct_modifyArrFxd (a,x) ==> 
+  modifyArrFxd (a,x) = (let (i,f,x) = x in modifyArrFxd (a,(0,f,x)))"
+  by (simp add: modifyArrFxd_def modifyArr'_def split_def Let_def fld_inverse)
 
 definition ctrct_modrefArrFxd :: "'arr \<times> ('m::len) word \<times> ('pel \<times> 'arg \<Rightarrow> 'pel \<times> 'out) \<times> 'arg \<Rightarrow> bool"
   where ctrct_modrefArrFxd_def[simp]:
-  "ctrct_modrefArrFxd x \<equiv> let (a,i,f,v) = x in vldFxd a (unat i)"
+  "ctrct_modrefArrFxd x \<equiv> let (a,(i,f,v)) = x in vldFxd a (unat i)"
 theorem sem_modrefArr:
- "ctrct_modrefArrFxd (a,i,f,x) \<Longrightarrow> 
-  modrefArrFxd (a,i,f,x) = 
-  (let (e,y) = f (toPtr (elmFxd (unat i) a), x) in (elm_updateFxd (unat i) (\<lambda>_.frPtr e) a, y))"
-  by (simp add: modrefArrFxd_def modrefArr'_def split_def Let_def vldArr lstFxd_def arrFxd_def elm_updateFxd_def elmFxd_def)
+ "ctrct_modrefArrFxd (a,x) \<Longrightarrow> 
+  modrefArrFxd (a,x) = 
+  (let (i,f,x) = x; (e,y) = f (toPtr (elmFxd (unat i) a), x) in (elm_updateFxd (unat i) (\<lambda>_.frPtr e) a, y))"
+  by (simp add: modrefArrFxd_def modrefArr'_def split_def Let_def elm_updateFxd_def elmFxd_def)
 theorem errsem_modrefArr:
- "\<not> ctrct_modrefArrFxd (a,i,f,x) ==> 
-  modrefArrFxd (a,i,f,x) = modrefArrFxd (a,0,f,x)"
-  by (simp add: modrefArrFxd_def modrefArr'_def vldArr fld_inverse)
+ "\<not> ctrct_modrefArrFxd (a,x) ==> 
+  modrefArrFxd (a,x) = (let (i,f,x) = x in modrefArrFxd (a,(0,f,x)))"
+  by (simp add: modrefArrFxd_def modrefArr'_def split_def Let_def fld_inverse)
 
 end
 
-text \<open>Extend the overloaded abstract data type to explicitly sized arrays.
-      Additionally introduce the following function for filling an array 
-      with an explicitly specified size.\<close>
-consts 
-  arr_fill_n :: "nat \<Rightarrow> (nat \<Rightarrow> 'el) \<Rightarrow> 'arr"
+subsection "Array Pointers and Pairs"
 
-text \<open>Wellformedness predicate for explicitly sized arrays:\<close>
-definition wlfES :: "'el CArrES\<^sub>T \<Rightarrow> bool"
-  where wlfES_def[simp]: "wlfES a \<equiv> 
-    length (fst a) = (unat (snd a)) \<and> length (fst a) > 0"
+text \<open>
+This corresponds to a direct application of the abstract data type to arbitrary lists.
+Additionally, an update function for pairs is defined. Together they are the basis
+for explicitly sized arrays.
+\<close>
 
-text \<open>Define the abstract data type functions for explicitly sized arrays.
-The explicit size is ignored and the intrinsic size of the list is used.\<close>
-definition sizES :: "'el CArrPtr\<^sub>T \<Rightarrow> nat"
-  where "sizES a \<equiv> length a"
-definition vldES :: "'el CArrPtr\<^sub>T \<Rightarrow> nat \<Rightarrow> bool"
-  where "vldES a i \<equiv> i < sizES a"
-definition elmES :: "nat \<Rightarrow> 'el CArrPtr\<^sub>T \<Rightarrow> 'el"
-  where "elmES i a \<equiv> nth a i"
-definition elm_updateES :: "nat \<Rightarrow> ('el \<Rightarrow> 'el) \<Rightarrow> 'el CArrPtr\<^sub>T \<Rightarrow> 'el CArrPtr\<^sub>T"
-  where "elm_updateES i f a \<equiv> (list_update a i (f (elmES i a)))"
-definition elm_modifiedES :: "nat \<Rightarrow> ('el \<Rightarrow> 'el \<Rightarrow> bool) \<Rightarrow> 'el CArrPtr\<^sub>T \<Rightarrow> 'el CArrPtr\<^sub>T \<Rightarrow> bool"
-  where elm_modified_defES: "elm_modifiedES i m a1 a2 \<equiv> 
-    m (elmES i a1) (elmES i a2) \<and> (\<forall>j \<noteq> i. vldES a1 j \<longrightarrow> elmES j a1 = elmES j a2)"
-definition arr_fill_nES :: "nat \<Rightarrow> (nat \<Rightarrow> 'el) \<Rightarrow> 'el CArrPtr\<^sub>T"
-  where "arr_fill_nES n f \<equiv> [f x . x \<leftarrow> [0 ..< n]]"
+text \<open>Define the abstract data type functions for lists.\<close>
 
-text \<open>Laws for the abstract data type functions\<close>
-lemma sizArrES: "sizES a = length a"
-  by (simp add:sizES_def)
-lemma vldArrES: "vldES a n = (n < length a)"
-  by (simp add: vldES_def sizArrES)
-lemma elm_identUpdES[simp]: "elm_updateES i (\<lambda>a. a) = (\<lambda>a. a)"
-  apply (unfold elm_updateES_def)
-  by(simp add: elmES_def)
-lemma elm_sameUpdES: "elm_updateES i (\<lambda>_. m (elmES i x)) x = elm_updateES i m x"
-  by(simp add: elm_updateES_def)
-thm list_update_same_conv
-lemma elm_distUpdES: "vldES a i \<Longrightarrow> (elm_updateES i f) ( (elm_updateES i g) a) = elm_updateES i (f \<circ> g) a"
-  for f:: "'el \<Rightarrow> 'el" and a::"'el CArrPtr\<^sub>T"
-  apply (unfold elm_updateES_def elmES_def fst_def vldArrES)
-  by(auto)
-lemma elm_commUpd_elmES: "i < j \<Longrightarrow> (elm_updateES j m2) \<circ> (elm_updateES i m1) = (elm_updateES i m1) \<circ> (elm_updateES j m2)"
-  apply (unfold elm_updateES_def elmES_def)
-  apply(rule ext,simp)
+definition sizPtr :: "'el CArrPtr\<^sub>T \<Rightarrow> nat"
+  where "sizPtr a \<equiv> length a"
+definition elmPtr :: "nat \<Rightarrow> 'el CArrPtr\<^sub>T \<Rightarrow> 'el"
+  where "elmPtr i a \<equiv> nth a i"
+definition elm_updatePtr :: "nat \<Rightarrow> ('el \<Rightarrow> 'el) \<Rightarrow> 'el CArrPtr\<^sub>T \<Rightarrow> 'el CArrPtr\<^sub>T"
+  (* Define elm_updatePtr as total, so that elm_distUpdPtr needs no assumption *)
+  where "elm_updatePtr i f a \<equiv> if i < length a then list_update a i (f (nth a i)) else a"
+definition elms_fill_nPtr :: "nat \<Rightarrow> (nat \<Rightarrow> 'el) \<Rightarrow> 'el CArrPtr\<^sub>T"
+  where "elms_fill_nPtr n f \<equiv> [f x . x \<leftarrow> [0 ..< n]]"
+
+text \<open>Define the function for updating the first component of a pair.\<close>
+
+definition fst_update :: "('a \<Rightarrow> 'a) \<Rightarrow> ('a \<times> 'b) \<Rightarrow> ('a \<times> 'b)"
+  where "fst_update f x = (f (fst x),snd x)"
+
+lemmas unfoldPtr = sizPtr_def elmPtr_def elm_updatePtr_def elms_fill_nPtr_def fst_update_def
+
+text \<open>Additional derived functions\<close>
+definition vldPtr :: "'el CArrPtr\<^sub>T \<Rightarrow> nat \<Rightarrow> bool"
+  where vldPtr_def[simp]: "vldPtr a i \<equiv> i < sizPtr a"
+definition elm_modifiedPtr :: "nat \<Rightarrow> ('el \<Rightarrow> 'el \<Rightarrow> bool) \<Rightarrow> 'el CArrPtr\<^sub>T \<Rightarrow> 'el CArrPtr\<^sub>T \<Rightarrow> bool"
+  where "elm_modifiedPtr i m a1 a2 \<equiv> 
+    m (elmPtr i a1) (elmPtr i a2) \<and> (\<forall>j \<noteq> i. vldPtr a1 j \<longrightarrow> elmPtr j a1 = elmPtr j a2)"
+lemmas elm_modified_defPtr = elm_modifiedPtr_def
+
+adhoc_overloading siz sizPtr
+  and vld vldPtr
+  and elm elmPtr
+  and elm_update elm_updatePtr
+  and elm_modified elm_modifiedPtr
+  and elms_fill_n elms_fill_nPtr
+
+definition fst_modified :: "('a \<Rightarrow> 'a \<Rightarrow> bool) \<Rightarrow> ('a \<times> 'b) \<Rightarrow> ('a \<times> 'b) \<Rightarrow> bool"
+  where "fst_modified m x1 x2 \<equiv> 
+    m (fst x1) (fst x2) \<and> (snd x1) = (snd x2)"
+
+text \<open>Simplification rules for selectors siz, elm, and fst\<close>
+lemma sizElmUpdPtr[simp]: "sizPtr (elm_updatePtr i f a) = sizPtr a"
+  by(simp add: unfoldPtr)
+lemma sizElmsFillPtr[simp]: "sizPtr (elms_fill_nPtr n f) = n"
+  by(simp add: unfoldPtr)
+lemma elmElmUpdPtr[simp]: "vldPtr a i \<Longrightarrow> elmPtr i (elm_updatePtr i f a) = f (elmPtr i a)"
+  by(simp add: unfoldPtr)
+lemma elmElmUpdFramePtr[simp]: "vldPtr a i \<and> vldPtr a j \<and> i \<noteq> j \<Longrightarrow> elmPtr j (elm_updatePtr i f a) = elmPtr j a"
+  by(simp add: unfoldPtr)
+lemma elmElmsFillPtr[simp]: "i < n \<Longrightarrow> elmPtr i (elms_fill_nPtr n f) = f i"
+  by(simp add: unfoldPtr)
+lemma fstFstUpd[simp]: "fst (fst_update f a) = f (fst a)"
+  by(auto simp add: fst_update_def)
+lemma fstFstUpdFrame[simp]: "snd (fst_update f a) = snd a"
+  by(auto simp add: fst_update_def)
+
+text \<open>Reasoning rules for elm_update and fst_update\<close>
+lemma elm_identUpdPtr[simp]: "elm_updatePtr i (\<lambda>a. a) = (\<lambda>a. a)"
+  by (rule ext,simp add: unfoldPtr)
+lemma elm_sameUpdPtr: "elm_updatePtr i (\<lambda>_. m (elmPtr i x)) x = elm_updatePtr i m x"
+  by(simp add: unfoldPtr)
+lemma elm_distUpdPtr: "(elm_updatePtr i f) \<circ> (elm_updatePtr i g) = elm_updatePtr i (f \<circ> g)"
+  by (rule ext,simp add: unfoldPtr)
+lemma elm_commUpd_elmPtr: "i < j \<Longrightarrow> (elm_updatePtr j m2) \<circ> (elm_updatePtr i m1) = (elm_updatePtr i m1) \<circ> (elm_updatePtr j m2)"
+  apply (unfold elm_updatePtr_def elmPtr_def)
+  apply(rule ext,simp,rule impI)
   apply(rule list_update_swap)
   by(simp)
-lemma elmElmUpdES: "vldES a i \<Longrightarrow> elmES i (elm_updateES i f a) = f (elmES i a)"
-  by(auto simp add: elm_updateES_def elmES_def vldArrES)
-lemma elmElmUpdFrameES: "vldES a i \<and> vldES a j \<and> i \<noteq> j \<Longrightarrow> elmES j (elm_updateES i f a) = elmES j a"
-  by(auto simp add: elm_updateES_def elmES_def vldArrES)
-lemma elmArrFillES: "i < n \<Longrightarrow> elmES i (arr_fill_nES n f) = f i"
-  by(auto simp add: elmES_def arr_fill_nES_def vldArrES)
-lemma sizArrFill: "sizES (arr_fill_nES n f) = n"
-  by(auto simp add: arr_fill_nES_def sizArrES)
+lemma fst_identUpd[simp]: "fst_update (\<lambda>a. a) = (\<lambda>a. a)"
+  apply (unfold fst_update_def)
+  by(simp)
+lemma fst_sameUpd: "fst_update (\<lambda>_. m (fst x)) x = fst_update m x"
+  by(simp add: fst_update_def)
+lemma fst_distUpd: "(fst_update f) \<circ> (fst_update g) = fst_update (f \<circ> g)"
+  apply (unfold fst_update_def)
+  by(auto)
 
 text \<open>Array equality by extensionality. \<close>
-lemma eqArrES: "sizES a1 = sizES a2 \<Longrightarrow>
+lemma eqArrPtr: "sizPtr a1 = sizPtr a2 \<Longrightarrow>
               (a1 = a2) = 
-              (\<forall> i. (vldES a1 i) \<longrightarrow> ((elmES i a1) = (elmES i a2)))"
+              (\<forall> i. (vldPtr a1 i) \<longrightarrow> ((elmPtr i a1) = (elmPtr i a2)))"
   for a1::"'el CArrPtr\<^sub>T" and a2::"'el CArrPtr\<^sub>T"
-  apply(rule iffI)
-   apply(rule allI)
-   apply(rule impI)
-   apply(auto simp add: elmES_def vldArrES sizArrES)
+  apply(rule iffI) apply(rule allI,rule impI)
+   apply(auto simp add: unfoldPtr)
   apply(case_tac a1)
   apply(case_tac a2)
   apply(auto)
   apply(rule nth_equalityI)
   by(auto)
 
-lemma eqElmUpdES: "sizES a1 = sizES a2 \<Longrightarrow> vldES a2 i \<Longrightarrow> (a1 = elm_updateES i f a2) =
-                 ((elmES i a1) = f (elmES i a2) \<and> (\<forall> j. j \<noteq> i \<and> (vldES a1 j) \<longrightarrow> (elmES j a1) = (elmES j a2)))"
-  apply(rule iffI)
-   apply(auto)
-    apply(subst elmElmUpdES,auto)
-  apply(subst elmElmUpdFrameES,auto simp add: vldArrES sizArrES)
-  apply(subst eqArrES)
-    apply(auto simp add:elm_updateES_def)
-   apply(auto simp add: elmES_def sizArrES)
+lemma eqElmUpdPtr: "sizPtr a1 = sizPtr a2 \<Longrightarrow> vldPtr a2 i \<Longrightarrow> (a1 = elm_updatePtr i f a2) =
+                 ((elmPtr i a1) = f (elmPtr i a2) \<and> (\<forall> j. j \<noteq> i \<and> (vldPtr a1 j) \<longrightarrow> (elmPtr j a1) = (elmPtr j a2)))"
+  apply(rule iffI,simp)
+  apply(simp add: eqArrPtr)
+  apply(rule allI)
   apply(case_tac "ia = i")
-   apply(simp)
-  by(auto simp add: vldArrES)
-lemma eqArrFillES: "sizES a = n \<Longrightarrow> (a = arr_fill_nES n f) = 
-                 ((\<forall> i. (vldES a i) \<longrightarrow> ((elmES i a) = f i)))"
-  apply(rule iffI)
-   apply(auto)
-   apply(rule elmArrFillES)
-   apply(simp add: vldArrES arr_fill_nES_def sizArrES)
-  apply(subst eqArrES)
-   apply(simp add: vldArrES arr_fill_nES_def sizArrES)
-   apply(simp add: arr_fill_nES_def)
-   apply(rule allI)
-   apply(rule impI)
-  by (auto simp add: elmES_def vldArrES sizArrES)
+   by(auto)
 
-text \<open>Semantics theorems for the Gencot array functions.\<close>
-lemma "a \<noteq> [] \<Longrightarrow> hd a = a ! 0"
-  sorry
+lemma eqElmsFillPtr: "sizPtr a = n \<Longrightarrow> (a = elms_fill_nPtr n f) = 
+                 ((\<forall> i. (vldPtr a i) \<longrightarrow> ((elmPtr i a) = f i)))"
+  apply(rule iffI,simp)
+  by(simp add: eqArrPtr)
+
+subsection "Explicitly Sized Arrays"
+
+text \<open>
+The abstract data type is applied to pairs consisting of a list and an explicit size.
+The explicit size is ignored and the intrinsic size of the list is used.
+\<close>
+
+text \<open>Define the abstract data type functions and a wellformedness predicate for pairs.\<close>
+
+definition sizES :: "'el CArrES\<^sub>T \<Rightarrow> nat"
+  where "sizES a \<equiv> sizPtr (fst a)"
+definition elmES :: "nat \<Rightarrow> 'el CArrES\<^sub>T \<Rightarrow> 'el"
+  where "elmES i a \<equiv> elmPtr i (fst a)"
+definition elm_updateES :: "nat \<Rightarrow> ('el \<Rightarrow> 'el) \<Rightarrow> 'el CArrES\<^sub>T \<Rightarrow> 'el CArrES\<^sub>T"
+  where "elm_updateES i f a \<equiv> fst_update (elm_updatePtr i f) a"
+definition elms_fill_nES :: "nat \<Rightarrow> (nat \<Rightarrow> 'el) \<Rightarrow> 'el CArrES\<^sub>T"
+  where "elms_fill_nES n f \<equiv> (elms_fill_nPtr n f,of_nat n)"
+definition wlfES :: "'el CArrES\<^sub>T \<Rightarrow> bool"
+  where "wlfES a \<equiv> sizPtr (fst a) = (unat (snd a)) \<and> sizPtr (fst a) > 0"
+
+lemmas unfoldES = sizES_def elmES_def elm_updateES_def elms_fill_nES_def wlfES_def
+
+text \<open>Additional derived functions\<close>
+definition vldES :: "'el CArrES\<^sub>T \<Rightarrow> nat \<Rightarrow> bool"
+  where vldES_def[simp]: "vldES a i \<equiv> i < sizES a"
+definition elm_modifiedES :: "nat \<Rightarrow> ('el \<Rightarrow> 'el \<Rightarrow> bool) \<Rightarrow> 'el CArrES\<^sub>T \<Rightarrow> 'el CArrES\<^sub>T \<Rightarrow> bool"
+  where "elm_modifiedES i m a1 a2 \<equiv> 
+    m (elmES i a1) (elmES i a2) \<and> (\<forall>j \<noteq> i. vldES a1 j \<longrightarrow> elmES j a1 = elmES j a2)"
+lemmas elm_modified_defES = elm_modifiedES_def
+
+adhoc_overloading siz sizES
+  and vld vldES
+  and elm elmES
+  and elm_update elm_updateES
+  and elm_modified elm_modifiedES
+  and elms_fill_n elms_fill_nES
+
+text \<open>Wellformedness implies nonempty and size limit\<close>
+
+lemma wlfsizES: "wlfES a \<Longrightarrow> sizES a > 0 \<and> sizES a < 2^64"
+  apply(cut_tac unat_lt2p[of "(snd a)"])
+  by(simp add: unfoldES)
+
+text \<open>Simplification rules for selectors siz and elm and the wellformedness predicate.\<close>
+
+lemma sizElmUpdES[simp]: "sizES (elm_updateES i f a) = sizES a"
+  by(simp add: unfoldES)
+lemma sizElmsFillES[simp]: "sizES (elms_fill_nES n f) = n"
+  by(simp add: unfoldES)
+lemma elmElmUpdES[simp]: "vldES a i \<Longrightarrow> elmES i (elm_updateES i f a) = f (elmES i a)"
+  by(simp add:unfoldES)
+lemma elmElmUpdFrameES[simp]: "vldES a i \<and> vldES a j \<and> i \<noteq> j \<Longrightarrow> elmES j (elm_updateES i f a) = elmES j a"
+  by(simp add:unfoldES)
+lemma elmElmsFillES[simp]: "i < n \<Longrightarrow> elmES i (elms_fill_nES n f) = f i"
+  by(simp add:unfoldES)
+lemma wlfElmUpdES[simp]: "wlfES (elm_updateES i f a) = wlfES a"
+  by(simp add: unfoldES)
+lemma wlfElmsFillES[simp]: "n > 0 \<and> n < 2^64 \<Longrightarrow> wlfES (elms_fill_nES n f)"
+  by(simp add: unfoldES unat_of_nat)
+
+text \<open>Reasoning rules for elm_update\<close>
+
+lemma elm_identUpdES[simp]: "elm_updateES i (\<lambda>a. a) = (\<lambda>a. a)"
+  by (rule ext,simp add: unfoldES)
+lemma elm_sameUpdES: "elm_updateES i (\<lambda>_. m (elmES i x)) x = elm_updateES i m x"
+  apply(simp add: unfoldES)
+  apply(subst fst_sameUpd[symmetric])
+  apply(subst elm_sameUpdPtr)
+  apply(subst fst_sameUpd)
+  by(simp)
+lemma elm_distUpdES: "(elm_updateES i f) \<circ> (elm_updateES i g) = elm_updateES i (f \<circ> g)"
+  for f:: "'el \<Rightarrow> 'el" and a::"'el CArrES\<^sub>T"
+  apply (rule ext,simp add: unfoldES)
+  apply(subst comp_apply[symmetric,where f="fst_update f" and g="fst_update g" for f g])
+  apply(subst fst_distUpd)
+  apply(subst elm_distUpdPtr)
+  by(simp)
+lemma elm_commUpd_elmES: "i < j \<Longrightarrow> (elm_updateES j m2) \<circ> (elm_updateES i m1) = (elm_updateES i m1) \<circ> (elm_updateES j m2)"
+  apply (unfold elm_updateES_def elmES_def)
+  apply(subst fst_distUpd)+
+  apply(subst elm_commUpd_elmPtr)
+  by(auto)
+
+text \<open>Array equality by extensionality. \<close>
+lemma eqArrES: "wlfES a1 \<and> wlfES a2 \<and> sizES a1 = sizES a2 \<Longrightarrow>
+              (a1 = a2) = 
+              (\<forall> i. (vldES a1 i) \<longrightarrow> ((elmES i a1) = (elmES i a2)))"
+  for a1::"'el CArrES\<^sub>T" and a2::"'el CArrES\<^sub>T"
+  apply(rule iffI,rule allI,rule impI)
+   apply(auto simp add: unfoldES)
+  apply(case_tac a1)
+  apply(case_tac a2)
+  by(auto simp add: eqArrPtr)
+
+lemma eqElmUpdES: 
+ "wlfES a1 \<and> wlfES a2 \<and> sizES a1 = sizES a2 \<and> vldES a2 i \<Longrightarrow> 
+  (a1 = elm_updateES i f a2) =
+  ((elmES i a1) = f (elmES i a2) \<and> (\<forall> j. j \<noteq> i \<and> (vldES a1 j) \<longrightarrow> (elmES j a1) = (elmES j a2)))"
+  apply(rule iffI,simp)
+  apply(simp add: eqArrES)
+  apply(rule allI)
+  apply(case_tac "ia = i")
+  by(auto)
+
+lemma eqElmsFillES: "wlfES a \<and> sizES a = n \<Longrightarrow> (a = elms_fill_nES n f) =
+                 ((\<forall> i. (vldES a i) \<longrightarrow> ((elmES i a) = f i)))"
+  apply(erule conjE)+
+  apply(frule wlfsizES)
+  apply(rule iffI,simp)
+  by(simp add: eqArrES)
+
+text \<open>Semantics theorems for the Gencot array operations.\<close>
+
 definition ctrct_getArrES :: "'el CArrES\<^sub>T \<times> ('m::len) word \<Rightarrow> bool"
   where ctrct_getArrES_def[simp]:
-  "ctrct_getArrES x \<equiv> let ((a,n),i) = x in (unat i) < (unat n)"
-theorem sem_getArrES: 
+    "ctrct_getArrES x \<equiv> let (a,i) = x in vldES a (unat i)"
+theorem sem_getArrES[sem]: 
  "wlfES a \<and> ctrct_getArrES (a,i) \<Longrightarrow> 
-  getArrES (a,i) = elmES (unat i) (fst a)"
-  by (auto simp add: getArrES_def elmES_def)
+  getArrES (a,i) = elmES (unat i) a"
+  by (simp add: getArrES_def Let_def split_def unfoldES unfoldPtr)
 theorem errsem_getArrES:
  "wlfES a \<and> \<not> ctrct_getArrES (a,i) \<Longrightarrow> 
-  getArrES (a,i) = elmES 0 (fst a)"
-  apply(simp add: getArrES_def vldArrES elmES_def split_def)
-  by(rule hd_conv_nth,simp)
+  getArrES (a,i) = elmES 0 a"
+  apply(erule conjE)+
+  apply(frule wlfsizES)
+  apply (simp add: getArrES_def Let_def split_def unfoldES unfoldPtr)
+  apply(rule hd_conv_nth)
+  by (simp)
 
 definition ctrct_setArrES :: "'el CArrES\<^sub>T \<times> ('m::len) word \<times> 'el \<Rightarrow> bool"
   where ctrct_setArrES_def[simp]:
-  "ctrct_setArrES x \<equiv> let ((a,n),i,v) = x in (unat i) < (unat n)"
-theorem sem_setArrES: 
+  "ctrct_setArrES x \<equiv> let (a,i,v) = x in vldES a (unat i)"
+theorem sem_setArrES[sem]: 
  "wlfES a \<and> ctrct_setArrES (a,i,v) \<Longrightarrow> 
-  setArrES (a,i,v) = ((elm_updateES (unat i) (\<lambda>_.v) (fst a),(snd a)), ())"
-  by (auto simp add: setArrES_def elm_updateES_def)
+  setArrES (a,i,v) = ((elm_updateES (unat i) (\<lambda>_.v) a), ())"
+  by (simp add: setArrES_def Let_def split_def unfoldES unfoldPtr)
 theorem errsem_setArrES:
  "wlfES a \<and> \<not> ctrct_setArrES (a,i,v) \<Longrightarrow> 
   setArrES (a,i,v) = (a,())"
-  by (simp add: setArrES_def split_def)
+  by (simp add: setArrES_def Let_def split_def unfoldES unfoldPtr)
 
 definition ctrct_modifyArrES :: "'el CArrES\<^sub>T \<times> ('m::len) word \<times> ('el \<times> 'arg \<Rightarrow> 'el \<times> 'out) \<times> 'arg \<Rightarrow> bool"
   where ctrct_modifyArrES_def[simp]:
-  "ctrct_modifyArrES x \<equiv> let ((a,n),i,f,v) = x in (unat i) < (unat n)"
-theorem sem_modifyArrES:
- "wlfES a \<and> ctrct_modifyArrES (a,i,f,x) \<Longrightarrow> 
-  modifyArrES (a,i,f,x) = 
-  (let (e,y) = f (elmES (unat i) (fst a), x) 
-  in ((elm_updateES (unat i) (\<lambda>_.e) (fst a),(snd a)), y))"
-  by (simp add: modifyArrES_def split_def Let_def elm_updateES_def elmES_def)
+  "ctrct_modifyArrES x \<equiv> let (a,(i,f,v)) = x in vldES a (unat i)"
+theorem sem_modifyArrES[sem]:
+ "wlfES a \<and> ctrct_modifyArrES (a,x) \<Longrightarrow> 
+  modifyArrES (a,x) = 
+  (let (i,f,x) = x; (e,y) = f (elmES (unat i) a, x) 
+  in ((elm_updateES (unat i) (\<lambda>_.e) a), y))"
+  by (simp add: modifyArrES_def Let_def split_def unfoldES unfoldPtr)
 theorem errsem_modifyArrES:
- "wlfES a \<and> \<not> ctrct_modifyArrES (a,i,f,x) ==> 
-  modifyArrES (a,i,f,x) = modifyArrES (a,0,f,x)"
-  by (simp add: modifyArrES_def split_def)
+ "wlfES a \<and> \<not> ctrct_modifyArrES (a,x) ==> 
+  modifyArrES (a,x) = (let (i,f,x) = x in modifyArrES (a,(0,f,x)))"
+  by (simp add: modifyArrES_def split_def unfoldES unfoldPtr)
 
 definition ctrct_modrefArrES :: "'el CArrES\<^sub>T \<times> ('m::len) word \<times> ('pel \<times> 'arg \<Rightarrow> 'pel \<times> 'out) \<times> 'arg \<Rightarrow> bool"
   where ctrct_modrefArrES_def[simp]:
-  "ctrct_modrefArrES x \<equiv> let ((a,n),i,f,v) = x in (unat i) < (unat n)"
-theorem sem_modrefArrES:
- "wlfES a \<and> ctrct_modrefArrES (a,i,f,x) \<Longrightarrow> 
-  modrefArrES (a,i,f,x) = 
-  (let (e,y) = f (toPtr (elmES (unat i) (fst a)), x) 
-  in ((elm_updateES (unat i) (\<lambda>_.frPtr e) (fst a),(snd a)), y))"
-  by (simp add: modrefArrES_def split_def Let_def elm_updateES_def elmES_def)
+  "ctrct_modrefArrES x \<equiv> let (a,(i,f,v)) = x in vldES a (unat i)"
+theorem sem_modrefArrES[sem]:
+ "wlfES a \<and> ctrct_modrefArrES (a,x) \<Longrightarrow> 
+  modrefArrES (a,x) = 
+  (let (i,f,x) = x; (e,y) = f (toPtr (elmES (unat i) a), x) 
+  in ((elm_updateES (unat i) (\<lambda>_.frPtr e) a), y))"
+  by (simp add: modrefArrES_def Let_def split_def unfoldES unfoldPtr)
 theorem errsem_modrefArrES:
- "wlfES a \<and> \<not> ctrct_modrefArrES (a,i,f,x) ==> 
-  modrefArrES (a,i,f,x) = modrefArrES (a,0,f,x)"
-  by (simp add: modrefArrES_def split_def)
+ "wlfES a \<and> \<not> ctrct_modrefArrES (a,x) ==> 
+  modrefArrES (a,x) = (let (i,f,x) = x in modrefArrES (a,(0,f,x)))"
+  by (simp add: modrefArrES_def split_def unfoldES unfoldPtr)
+
+subsection "Array Conversion Functions"
+
+context CArrLems
+begin
+
+text \<open>Semantics theorems.\<close>
+
+theorem sem_toCAES:
+ "toCAESFxd a = elms_fill_nES (sizFxd a) (\<lambda>i. elmFxd i a)"
+  apply(simp add: toCAESFxd_def toCAES'_def unfoldES unfoldPtr unfold)
+  apply(subst map_nth[symmetric])
+  by(simp add: length_FixedList)
+
+theorem sem_fromCAES:
+ "sizES a = LENGTH('n) \<Longrightarrow> 
+  fromCAESFxd a = elms_fillFxd (\<lambda>i. elmES i a)"
+  apply(simp add: fromCAESFxd_def fromCAES'_def unfoldES unfoldPtr unfold) 
+  apply(subst map_nth[symmetric])
+  by(auto)
+
+theorem sem_rotoCAES[simp]: "rotoCAESFxd = toCAESFxd"
+  apply(rule ext)
+  by(simp add: rotoCAESFxd_def toCAESFxd_def)
+
+theorem sem_rofromCAES[simp]: "rofromCAESFxd = fromCAESFxd"
+  apply(rule ext)
+  by(simp add: rofromCAESFxd_def fromCAESFxd_def)
+
+text \<open>
+The following rules can be used for simplifying reasoning when the semantics
+is applied by omitting the semantics of the conversion functions.
+\<close>
+
+text \<open>Simplification rules for selectors siz and elm and the wellformedness predicate.\<close>
+
+lemma sizToCAES[simp]: 
+ "sizES (toCAESFxd a) = sizFxd a"
+  by(simp add: sem_toCAES)
+lemma elmToCAES[simp]:
+ "vldFxd a i \<Longrightarrow> elmES i (toCAESFxd a) = elmFxd i a"
+  by(simp add: sem_toCAES)
+lemma wlfToCAES[simp]:
+ "sizFxd a < 2^64 \<Longrightarrow> wlfES (toCAESFxd a)"
+  by(simp add: sem_toCAES)
+lemma sizFromCAES[simp]: 
+ "sizES a = LENGTH('n) \<Longrightarrow> 
+  sizFxd (fromCAESFxd a) = sizES a"
+  by(simp)
+lemma elmFromCAES[simp]:
+ "sizES a = LENGTH('n) \<and> vldES a i \<Longrightarrow> 
+  elmFxd i (fromCAESFxd a) = elmES i a"
+  by(simp add: sem_fromCAES)
+
+text \<open>Inversion rules for the conversion functions.\<close>
+lemma toCAES_inverse: 
+ "fromCAESFxd (toCAESFxd a) = a"
+  apply(rule sym)
+  by(simp add: sem_toCAES sem_fromCAES eqElmsFill)
+
+lemma fromCAES_inverse: 
+ "wlfES a \<and> sizES a = LENGTH('n) \<Longrightarrow>
+  toCAESFxd (fromCAESFxd a) = a"
+  apply(rule sym)
+  by(simp add: sem_toCAES sem_fromCAES eqElmsFillES)
+
+text \<open>Rules for applying the conversion functions.\<close>
+
+lemma fromCAESElmUpd:
+ "vld a i \<and> sizES a = LENGTH('n) \<Longrightarrow>
+  fromCAESFxd (elm_updateES i m a) = elm_updateFxd i m (fromCAESFxd a)"
+  by(simp add: sem_fromCAES eqElmUpd)
+lemma fromCAESElmsFill:
+ "n = LENGTH('n) \<Longrightarrow>
+  fromCAESFxd (elms_fill_nES n f) = elms_fillFxd f"
+  by(simp add: sem_fromCAES eqElmsFill)
+lemmas fromCAES_apply = fromCAESElmUpd fromCAESElmsFill
+
+lemma toCAESElmUpd:
+ "sizFxd a < 2^64 \<and> vldFxd a i \<Longrightarrow>
+  toCAESFxd (elm_updateFxd i m a) = elm_updateES i m (toCAESFxd a)"
+  by(simp add: sem_toCAES eqElmUpdES)
+lemma toCAESElmsFill:
+ "n < 2^64 \<and>n = LENGTH('n) \<Longrightarrow>
+  toCAESFxd (elms_fillFxd f) = elms_fill_n n f"
+  by(simp add: sem_toCAES eqElmsFillES)
+lemmas toCAES_apply = toCAESElmUpd toCAESElmsFill
+
+end
 
 end
